helping/elim_stack/StackIA.v
@@ -1,6 +1,6 @@
 Require Import CRIS.
 Require Import ImpPrelude.
-Require Import MemTactics.
+Require Import MemTactics MemA.
 Require Import SchHeader SchI SchA SchTactics.
 Require Import StackHeader StackA StackI.
 From CRIS.helping Require Import Header HelpingOn HelpingOnOffproof HelpingTactics.
@@ -61,18 +61,21 @@ Module StackIM. Section StackIM.
   Qed.
   Hint Resolve yield_msk alloc_msk store_msk load_msk cas_msk cmp_msk : core.
 
-  Definition init_cond : iProp Σ := emp%I.
+  Definition init_cond : iProp Σ := helping_auth 1 ∅%I.
 
   Local Definition MemA := MemA.t.
   Local Definition SchI := CFilter.filter msk SchI.t.
-  Local Definition HelpingOn := HelpingOn.t mn StackM.jobCode StackM.retCode sp.
-  Local Definition StackM := (StackM.t mn N sp ★ MemA) ★ HelpingOn ★ SchI.
-  Local Definition StackI := CFilter.filter msk (StackI.t ★ MemA) ★ SchI.
-  Local Definition IstFull :=
-    (IstHelp StackM.jobID StackM.retID mn (IstProd ((IstSB (Mod.scopes StackM) IstTrue)) IstEq)).
+  Local Definition HelpingOn := HelpingOn.t mn StackM.jobCode sp.
+  Local Definition StackM := (StackM.t mn N sp ★ MemA)            ★ SchI ★ HelpingOn.
+  Local Definition StackI := CFilter.filter msk (StackI.t ★ MemA) ★ SchI ★ HelpingOn.
 
-  Let offerN := N .@ "offer".
-  Let stackN := N .@ "stack".
+  Definition IstHelp : ist_type Σ := λ st_src st_tgt,
+    (∃ (reqmap_s reqmap_t : gmap nat (option retID * jobID)),
+      ⌜st_src = [(HelpingOn.v_reqs mn, reqmap_s↑)] ∧
+       st_tgt = [(HelpingOn.v_reqs mn, reqmap_t↑)]⌝ ∗
+      helping_auth 1 reqmap_s)%I.
+
+  Local Definition IstFull := IstProd (IstSB (Mod.scopes StackM) IstTrue) IstHelp.
 
   Lemma new_stack_simF :
     ISim.sim_fun open StackM StackI init_cond IstFull (Some StackHdr.new_stack).
@@ -103,16 +106,17 @@ Module StackIM. Section StackIM.
       [try prove_inline_cond|try prove_sb_cond|..|unfold_cris_defs].
     iIntros "↦val". steps_r. hss_r.
 
-    steps_r. sch_yield_ir.
-    steps_r.
+    steps_r. sch_yield_ir. steps_r.
 
+    (* Guarantee the postcondition *)
     sch_yield_l.
     iMod (own_alloc (● Excl' [] ⋅ ◯ Excl' [])) as (γs) "[Hs● Hs◯]".
     { apply auth_both_valid_discrete. split; done. }
-    iMod (inv_alloc (syn_stack_inv N γs stackb 0%Z 0) _ _ _ stackN with "[-Hs◯ IST TID]")
+    iMod (inv_alloc (syn_stack_inv N γs stackb 0%Z 0) _ _ _ (stackN N) with "[-Hs◯ IST TID]")
       as "#Hinv"; eauto.
     { apply nclose_subseteq. }
-    { rewrite /syn_stack_inv /syn_is_offer SLRed_red. iExists (Vint 0), (Vint 0), []; iFrame; eauto.
+    { rewrite /syn_stack_inv /syn_is_offer SLRed_red. iLeft.
+      iExists (Vint 0), (Vint 0), []; iFrame; eauto.
       rewrite SLRed_red //.
     }
 
@@ -140,9 +144,26 @@ Module StackIM. Section StackIM.
 
     (* Register for helping *)
     steps_r. norm_l.
-    iApply (wsim_helping_run with "IST");
-      [try prove_inline_cond|try prove_sb_cond|unfold_cris_defs|..].
-    clear st_src st_tgt; iIntros (st_src st_tgt req_id) "IST Help".
+
+    (* TODO : factor out this proof into a lemma *)
+    inline_l. steps_l. hss.
+    iDestruct "IST" as "[% [% [% [% [[-> ->] [IST [% [% [[-> ->] Help●]]]]]]]]]". steps_l. hss.
+    rename _q into reqmap_s.
+    iMod (own_update with "Help●") as "[Help● Help◯]".
+    { eapply (gmap_view_alloc _ (fresh (dom reqmap_s)) (DfracOwn 1)); eauto.
+      { apply not_elem_of_dom. rewrite dom_fmap. apply is_fresh. }
+      { rewrite dfrac_valid; eauto. }
+      { instantiate (1:=(to_agree (None, _))); ss. }
+    }
+    set (st_src := st_srcL ++ _). set (st_tgt := st_tgtL ++ _).
+    iAssert (IstFull st_src st_tgt)%I with "[IST Help●]" as "IST".
+    { iFrame. subst st_src. ss. iExists _, _; iSplit; first done.
+      rewrite -fmap_insert //. iExists _, _; iFrame; done.
+    }
+    iAssert (helping_token (fresh (dom _)) _)%I with "Help◯" as "Tkn".
+    generalize (fresh (dom reqmap_s)) as req_id; intros req_id.
+    generalize (st_src); clear st_src; intros st_src.
+    generalize (st_tgt); clear st_tgt; intros st_tgt.
 
     (* Coinduction starts here *)
     iApply wsim_reset. iStopProof.
@@ -159,7 +180,11 @@ Module StackIM. Section StackIM.
     (* load *)
     iInv "Hinv" as "Hstack" "close".
     rewrite {1}SLRed_red.
-    iDestruct "Hstack" as "[%stack_rep [%offer_rep [%l [Hs [H↦ [Hlist Hoffer]]]]]]".
+    iDestruct "Hstack" as "[[%stack_rep [%offer_rep [%l [Hs [H↦ [Hlist Hoffer]]]]]]|[% ●]]";
+      cycle 1.
+    { iExFalso. iDestruct "IST" as "[% [% [% [% [% [? [% [% [IST ●2]]]]]]]]]".
+      iCombine "●" "●2" gives %[WF _]%gmap_view_auth_dfrac_op_valid. ss.
+    }
 
     iApply (wsim_mem_load with "[H↦]");
       [try prove_inline_cond|try prove_sb_cond|ss|unfold_cris_defs].
@@ -167,8 +192,8 @@ Module StackIM. Section StackIM.
 
     iPoseProof (list_inv_comparable with "Hlist") as "[Hlist [Hval #Hcomp]]".
     iMod ("close" with "[Hs Hlist H↦ Hoffer]") as "_".
-    { rewrite /syn_stack_inv /syn_is_offer.
-      do 3 (SL_red; iExists _); SL_red; iFrame. rewrite SLRed_red //.
+    { rewrite /syn_stack_inv. SL_red; iLeft.
+      do 3 (iExists _; SL_red). SL_red; iFrame. rewrite SLRed_red //.
     }
 
     (* alloc new head *)
@@ -189,7 +214,11 @@ Module StackIM. Section StackIM.
     sch_yield_ir. steps_r.
     iInv "Hinv" as "Hstack" "close".
     rewrite SLRed_red.
-    iDestruct "Hstack" as "[%stack_rep' [%offer_rep' [%l' [Hs [H↦ [Hlist Hoffer]]]]]]".
+    iDestruct "Hstack" as "[[%stack_rep' [%offer_rep' [%l' [Hs [H↦ [Hlist Hoffer]]]]]]|[% ●]]";
+      cycle 1.
+    { iExFalso. iDestruct "IST" as "[% [% [% [% [% [? [% [% [IST ●2]]]]]]]]]".
+      iCombine "●" "●2" gives %[WF _]%gmap_view_auth_dfrac_op_valid. ss.
+    }
     iPoseProof (list_inv_comparable with "Hlist") as "[Hlist [Hval2 _]]".
     iPoseProof ("Hcomp" with "Hlist") as "[%succ %Hcomp]".
 
@@ -206,10 +235,10 @@ Module StackIM. Section StackIM.
       (* atomic update happens here: since it is valid to update stack_contents here (without any
          helps from other threads), the pusher does its own job *)
       sch_yield_l. norm_l.
-      iApply (wsim_helping_try_run with "Help IST").
-      clear st_src; iIntros (reqmap st_src) "Help IST".
-      rewrite /StackM.jobCode /=. steps_l.
-      rewrite Helping.trans_take. steps_l. clear l; rename _q into l.
+      rewrite /HelpingOn.try_run.
+      iDestruct "IST" as "[% [% [% [% [[-> ->] [IST [% [% [[-> ->] Help●]]]]]]]]]". steps_l. hss.
+      iPoseProof (helping_auth_token with "Help● Help") as "%Hlookup"; rewrite Hlookup /=.
+      rewrite Helping.trans_take. steps_l. clear l; rename _q0 into l.
       rewrite Helping.trans_Assume. steps_l.
       iCombine "Hs ASM" gives
         %[->%Excl_included%leibniz_equiv _]%auth_both_valid_discrete.
@@ -220,15 +249,19 @@ Module StackIM. Section StackIM.
 
       (* we updated the user-side resource, now proceed *)
       iMod ("close" with "[Hnewv Hnewhead Hoffer Hlist H↦ Hs]") as "_".
-      { iExists _, offer_rep', (v :: l'). iFrame. iExists 1%Qp; iSplit; eauto.
+      { iLeft. iExists _, offer_rep', (v :: l'). iFrame. iExists 1%Qp; iSplit; eauto.
         rewrite Z.add_0_l.
         destruct stack_rep, stack_rep'; inv Hcomp; des_ifs.
         simpl_bool; des; do 2 destruct (dec _ _); clarify.
       }
-      iMod (IstHelp_done with "Help IST") as "[Done IST]".
+      (* restoring IST *)
+      iMod (helping_auth_commit with "Help● Help") as "[Help● Help◯]".
+      clear st_src st_tgt. set (st_src := st_srcL0 ++ _); set (st_tgt := st_tgtL0 ++ _).
+      iAssert (IstFull st_src st_tgt)%I with "[IST Help●]" as "IST".
+      { iExists _, _, _, _; iFrame "Help●". iSplit; eauto. }
 
       (* comparison *)
-      sch_yield_ir. steps_r.
+      sch_yield_ir. clear st_src st_tgt. steps_r.
       iCombine "Hval" "Hval2" as "Hval".
       iApply (wsim_mem_cmp with "Hval");
         [try prove_inline_cond|try prove_sb_cond|unfold_cris_defs|..]; eauto.
@@ -245,7 +278,7 @@ Module StackIM. Section StackIM.
     (* failure *)
     steps_r. hss_r. steps_r.
     iMod ("close" with "[Hnewv Hnewhead Hoffer Hlist H↦ Hs]") as "_".
-    { iExists _, offer_rep', l'. iFrame. }
+    { iLeft. iExists _, offer_rep', l'. iFrame. }
 
     (* comparison - which leads us to offering *)
     sch_yield_ir. steps_r.
@@ -279,45 +312,54 @@ Module StackIM. Section StackIM.
     sch_yield_ir; steps_r.
     iInv "Hinv" as "Hstack" "close".
     rewrite {1}SLRed_red. clear dependent l l' stack_rep stack_rep' offer_rep offer_rep'.
-    iDestruct "Hstack" as "[%stack_rep [%offer_rep [%l [Hs [H↦ [Hlist [Hoffer↦ _]]]]]]]".
+    iDestruct "Hstack" as "[[%stack_rep [%offer_rep [%l [Hs [H↦ [Hlist [Hoffer↦ _]]]]]]]|[% ●]]";
+      cycle 1.
+    { iExFalso. iDestruct "IST" as "[% [% [% [% [% [? [% [% [IST ●2]]]]]]]]]".
+      iCombine "●" "●2" gives %[WF _]%gmap_view_auth_dfrac_op_valid. ss.
+    }
+
     iApply (wsim_mem_store with "Hoffer↦");
       [try prove_inline_cond|try prove_sb_cond|unfold_cris_defs].
     iIntros "Hoffer↦". steps_r. hss_r.
     iMod (own_alloc (Excl ())) as "[%γo OfferTkn]"; ss.
     iMod (inv_alloc
-      (syn_offer_inv 0 γo (offerb, 0%Z) (stid, mtid, (Vptr (stackb, stackofs), v, γs)))
-      _ _ _ offerN with "[Hofferv Hofferst Help]") as "#Hoinv"; eauto.
+      (syn_offer_inv 0 γo (offerb, 0%Z) req_id (stid, mtid, (Vptr (stackb, stackofs), v, γs)))
+      _ _ _ (offerN N) with "[Hofferv Hofferst Help]") as "#Hoinv"; eauto.
     { apply nclose_subseteq. }
-    { rewrite SLRed_red; iExists _, _; iFrame. done. }
+    { rewrite SLRed_red; iExists _; iFrame. done. }
 
     iMod ("close" with "[Hoffer↦ Hlist H↦ Hs]") as "_".
-    { rewrite SLRed_red. iExists _, (Vptr (offerb, 0%Z)), l. iFrame.
-      rewrite /syn_is_offer /= SLRed_red. iExists γo, _. rewrite inv_red //. }
+    { rewrite SLRed_red. iLeft. iExists _, (Vptr (offerb, 0%Z)), l. iFrame.
+      rewrite /syn_is_offer /= SLRed_red. iExists γo, _, _. rewrite inv_red; iSplit; eauto.
+    }
     steps_r. sch_yield_ir. steps_r.
 
     iInv "Hinv" as "Hstack" "close".
     rewrite {1}SLRed_red. clear dependent l stack_rep offer_rep.
-    iDestruct "Hstack" as "[%stack_rep [%offer_rep [%l [Hs [H↦ [Hlist [Hoffer↦ _]]]]]]]".
+    iDestruct "Hstack" as "[[%stack_rep [%offer_rep [%l [Hs [H↦ [Hlist [Hoffer↦ _]]]]]]]|[% ●]]";
+      cycle 1.
+    { iExFalso. iDestruct "IST" as "[% [% [% [% [% [? [% [% [IST ●2]]]]]]]]]".
+      iCombine "●" "●2" gives %[WF _]%gmap_view_auth_dfrac_op_valid. ss.
+    }
     iApply (wsim_mem_store with "Hoffer↦");
       [try prove_inline_cond|try prove_sb_cond|unfold_cris_defs].
     iIntros "Hoffer↦". steps_r. hss_r.
 
     iMod ("close" with "[Hoffer↦ Hlist H↦ Hs]") as "_".
-    { rewrite SLRed_red. iExists _, _, l. iFrame. rewrite SLRed_red //. }
+    { rewrite SLRed_red. iLeft. iExists _, _, l. iFrame. rewrite SLRed_red //. }
     steps_r. sch_yield_ir. steps_r.
 
     iInv "Hoinv" as "oinv" "close"; rewrite {1}SLRed_red.
-    iDestruct "oinv" as "[%offerst [%rid [offerv↦ [offerst↦ offer]]]] /=".
+    iDestruct "oinv" as "[%offerst [offerst↦ offer]] /=".
     rewrite Z.add_0_l.
-    destruct offerst; try by (iCombine "OfferTkn" "offer" gives %WF).
-    destruct n; try by (iCombine "OfferTkn" "offer" gives %WF).
+    case_decide; subst.
     { (* nobody helped*)
       iApply (wsim_mem_cas _ _ _ _ _ _ _ _ _ _ _ _ _ _ _ _ emp%I with "offerst↦");
         [try prove_inline_cond|try prove_sb_cond|unfold_cris_defs|..]; eauto.
       des_ifs_safe. iIntros "Hofferst _". steps_r. hss_r. steps_r.
 
-      iMod ("close" with "[offerv↦ Hofferst OfferTkn]") as "_".
-      { rewrite SLRed_red. iExists _, _. iFrame. done. }
+      iMod ("close" with "[Hofferst OfferTkn]") as "_".
+      { rewrite SLRed_red. iExists _. iFrame. done. }
 
       steps_r. sch_yield_ir. steps_r.
       iAssert (emp)%I as "E"; first done.
@@ -325,11 +367,36 @@ Module StackIM. Section StackIM.
         [try prove_inline_cond|try prove_sb_cond|unfold_cris_defs|..]; eauto.
       iIntros "_". steps_r. hss_r. steps_r.
 
-      by_coind CIH. iFrame.
-      (* TODO : make request id explicit in the invariant *)
-      admit.
+      by_coind CIH. iDestruct "offer" as "[? ?]"; iFrame. done.
     }
-    (* Helped! *)
+    case_decide; subst.
+    { (* Somebody helped *)
+      iApply (wsim_mem_cas _ _ _ _ _ _ _ _ _ _ _ _ _ _ _ _ emp%I with "offerst↦");
+        [try prove_inline_cond|try prove_sb_cond|unfold_cris_defs|..]; eauto.
+      des_ifs_safe. iIntros "Hofferst _". steps_r. hss_r. steps_r.
+      iPoseProof "offer" as "#offer".
+
+      iMod ("close" with "[Hofferst]") as "_".
+      { rewrite SLRed_red. iExists _. iFrame. done. }
+
+      sch_yield_ir. steps_r.
+      iAssert (emp)%I as "E"; first done.
+      iApply (wsim_mem_cmp with "E");
+        [try prove_inline_cond|try prove_sb_cond|unfold_cris_defs|..]; eauto.
+      iIntros "_". steps_r. hss_r. steps_r.
+
+      sch_yield_l.
+      rewrite /HelpingOn.try_run /=. steps_l.
+      iDestruct "IST" as "[% [% [% [% [[-> ->] [? [% [% [[-> ->] Help●]]]]]]]]]".
+      steps_l. hss.
+
+      iPoseProof (helping_auth_done with "Help● offer") as "[% %Heq]"; rewrite Heq; clear Heq.
+      steps_l. sch_yield_l. steps_l. force_l. hss. iFrame. iSplit; eauto.
+      step. iFrame. iSplit; eauto.
+    }
+
+    case_decide; try by (iCombine "OfferTkn" "offer" gives %WF). ss.
+  Unshelve. all: try exact 1%Qp.
   (*SLOW*)Admitted.
 
   Lemma pop_simF : ISim.sim_fun open StackM StackI init_cond IstFull (Some StackHdr.pop).
@@ -351,8 +418,12 @@ Module StackIM. Section StackIM.
 
     (* Stack load *)
     iInv "Hinv" as "Hstack" "close".
-    rewrite SLRed_red.
-    iDestruct "Hstack" as "[%stack_rep [%offer_rep [%l [Hs [H↦ [Hlist Hoffer]]]]]]".
+    rewrite {1}SLRed_red.
+    iDestruct "Hstack" as "[[%stack_rep [%offer_rep [%l [Hs [H↦ [Hlist Hoffer]]]]]]|[% ●]]";
+      cycle 1.
+    { iExFalso. iDestruct "IST" as "[% [% [% [% [% [? [% [% [IST ●2]]]]]]]]]".
+      iCombine "●" "●2" gives %[WF _]%gmap_view_auth_dfrac_op_valid. ss.
+    }
 
     iApply (wsim_mem_load with "[H↦]");
       [try prove_inline_cond|try prove_sb_cond|ss|unfold_cris_defs].
@@ -360,33 +431,240 @@ Module StackIM. Section StackIM.
 
     destruct (decide (stack_rep = Vint 0%Z)); subst.
     { (* Empty stack - terminate *)
-      sch_yield_l. steps_l.
-      destruct Hsphelp as [Hfind2 Hfind]; rewrite (Hfind (Helping.help mn) None) //; cycle 1.
-      { rewrite /alist_find eq_rel_dec_correct /=; des_ifs; destruct (dec _ _); ss. }
-      clear Hfind Hfind2.
+      sch_yield_l. steps_l. force_l false. steps_l.
 
-      iDestruct "IST" as "[% [% [-> [Help● IST]]]]".
-      inline_l. steps_l. force_l (fresh (dom reqmap)). steps_l.
-      rewrite /HoareCall_prologue; unseal "Help".
-      unfold_sp_exact sp (SchHdr.yield); ss.
-      force_l (stid, mtid). steps_l.
-      force_l (()↑).
-      iDestruct "Help●" as "[Help● Help●2]".
-      force_l.
-      admit. 
+      (* Atomic update *)
+      iCombine "Hs ASM" gives %[->%Excl_included%leibniz_equiv _]%auth_both_valid_discrete.
+      destruct l; [|ss; iPoseProof "Hlist" as "[% [% [% [% [% [% ?]]]]]]"; clarify].
+      force_l. iFrame. steps_l.
+
+      iMod ("close" with "[Hs Hlist Hoffer H↦]") as "_".
+      { rewrite /syn_stack_inv SLRed_red. SL_red; iLeft.
+        do 3 (iExists _; SL_red). SL_red; iFrame. rewrite SLRed_red //.
+      }
+      sch_yield_ir. steps_r. sch_yield_l. force_l. iFrame. iSplit; eauto. step. iSplit; done.
     }
+    (* Stack nonempty *)
     iPoseProof (list_inv_comparable with "Hlist") as "[Hlist [Hval #Hcomp]]".
-    admit.
-  Admitted.
+
+    destruct l as [|v l]; ss; first iPoseProof "Hlist" as "%"; clarify.
+    iDestruct "Hlist" as (headb headofs stackrep q0 q1) "[-> [↦v [↦next Hlist]]]".
+    iDestruct "↦next" as "[↦next ↦next2]".
+    iMod ("close" with "[Hs Hlist H↦ ↦v ↦next2 Hoffer]") as "_".
+    { rewrite /syn_stack_inv. SL_red; iLeft.
+      do 3 (iExists _; SL_red). SL_red; iFrame. rewrite SLRed_red //=.
+      iExists _, _, _, _; iFrame; eauto.
+    }
+
+    sch_yield_ir. steps_r. sch_yield_ir. steps_r.
+    iApply (wsim_mem_load with "[↦next]");
+      [try prove_inline_cond|try prove_sb_cond|ss|unfold_cris_defs]; eauto.
+    iIntros "↦next". steps_r. hss_r. steps_r. sch_yield_ir. steps_r.
+
+    iInv "Hinv" as "Hstack" "close".
+    rewrite {1}SLRed_red.
+    iDestruct "Hstack" as "[[%stack_rep' [%offer_rep' [%l' [Hs [H↦ [Hlist Hoffer]]]]]]|[% ●]]";
+      cycle 1.
+    { iExFalso. iDestruct "IST" as "[% [% [% [% [% [? [% [% [IST ●2]]]]]]]]]".
+      iCombine "●" "●2" gives %[WF _]%gmap_view_auth_dfrac_op_valid. ss.
+    }
+    iPoseProof (list_inv_comparable with "Hlist") as "[Hlist [Hval2 _]]".
+    iPoseProof ("Hcomp" with "Hlist") as "[%succ %Hcomp]".
+
+    iCombine "Hval Hval2" as "Hcmp".
+    iApply (wsim_mem_cas with "H↦ Hcmp");
+      [try prove_inline_cond|try prove_sb_cond|unfold_cris_defs|..]; eauto.
+    { iIntros "[[% [% $]] [% [% $]]] !> [$ $] //". }
+    iIntros "H↦ [Hval Hval2]". iClear "Hcomp". steps_r. hss_r. steps_r.
+    case_decide; subst.
+    { (* Pop success *)
+      sch_yield_l. steps_l. force_l false. steps_l.
+      destruct (stack_rep') as [[| |]|[bold ofsold]|]; inv Hcomp; do 2 destruct (dec _ _); ss.
+      destruct l'; ss.
+      { iPoseProof "Hlist" as "%"; ss. }
+      iDestruct "Hlist" as "[% [% [% [% [% [% [Hpt1 [Hpt2 Hlist]]]]]]]]". clarify.
+      iPoseProof (mem_points_to_singleton_agree with "↦next Hpt2") as "<-".
+      iCombine "Hs ASM" gives %[->%Excl_included%leibniz_equiv _]%auth_both_valid_discrete.
+      iMod (own_update_2 with "Hs ASM") as "[Hs ASM]".
+      { eapply auth_update, option_local_update, (exclusive_local_update _ (Excl _)). done. }
+      force_l; iFrame. steps_l.
+      iMod ("close" with "[Hs Hlist H↦ Hoffer]") as "_".
+      { rewrite (SLRed_red (f := syn_stack_inv _ _ _ _ _)). iLeft. iFrame. }
+      sch_yield_ir. steps_r.
+
+      iCombine "Hval Hval2" as "Hval".
+      iApply (wsim_mem_cmp with "Hval");
+        [try prove_inline_cond|try prove_sb_cond|unfold_cris_defs|..]; eauto.
+      { do 2 destruct (dec _ _); ss. }
+      { iIntros "[[% [% $]] [% [% $]]] !> [$ $] //". }
+      iIntros "[[% [% Hval]] _]". steps_r. hss_r. steps_r. sch_yield_ir. steps_r.
+      iApply (wsim_mem_load with "[Hval]");
+        [try prove_inline_cond|try prove_sb_cond|ss|unfold_cris_defs].
+      iIntros "[Hpt3 _]".
+      iPoseProof (mem_points_to_singleton_agree with "Hpt3 Hpt1") as "<-".
+      steps_r. hss_r. steps_r. sch_yield_ir. steps_r.
+      sch_yield_l. force_l. iFrame. iSplit; eauto. step. iFrame. eauto.
+    }
+
+    (* Pop failure *)
+    iMod ("close" with "[↦next Hs Hoffer Hlist H↦]") as "_".
+    { rewrite (SLRed_red (f:=syn_stack_inv _ _ _ _ _)). iLeft. iFrame. }
+    sch_yield_ir. steps_r.
+    iCombine "Hval Hval2" as "Hval".
+    iApply (wsim_mem_cmp with "Hval");
+      [try prove_inline_cond|try prove_sb_cond|unfold_cris_defs|..]; eauto.
+    { iIntros "[[% [% $]] [% [% $]]] !> [$ $] //". }
+    iIntros "_". steps_r. hss_r. steps_r.
+    assert (succ = 0%Z); last subst succ.
+    { destruct stack_rep' as [[|?|?]|[? ?]|]; inv Hcomp; ss; do 2 destruct (dec _ _); ss; clarify. }
+    steps_r. sch_yield_ir. steps_r.
+
+    (* Check the offer *)
+    iInv "Hinv" as "Hstack" "close".
+    rewrite {1}SLRed_red. clear dependent stack_rep' offer_rep offer_rep' l  l'.
+    iDestruct "Hstack" as "[[%stack_rep [%offer_rep [%l [Hs [H↦ [Hlist Hoffer]]]]]]|[% ●]]";
+      cycle 1.
+    { iExFalso. iDestruct "IST" as "[% [% [% [% [% [? [% [% [IST ●2]]]]]]]]]".
+      iCombine "●" "●2" gives %[WF _]%gmap_view_auth_dfrac_op_valid. ss.
+    }
+    iDestruct "Hoffer" as "[↦offer Hoffer]".
+    iApply (wsim_mem_load with "↦offer");
+      [try prove_inline_cond|try prove_sb_cond|unfold_cris_defs|..]; eauto.
+    iIntros "↦offer". steps_r. hss_r. steps_r.
+    rewrite /syn_is_offer; destruct (offer_rep) as [[|?|?]|[offerb offerofs]|]; rewrite SLRed_red;
+      try iPoseProof ("Hoffer") as "%"; ss.
+    { steps_r.
+      iMod ("close" with "[Hs H↦ Hlist ↦offer]") as "_".
+      { rewrite (SLRed_red (f:=syn_stack_inv _ _ _ _ _)). iLeft; iFrame.
+        rewrite /syn_is_offer SLRed_red //.
+      }
+      by_coind CIH. iFrame. done.
+    }
+    iDestruct "Hoffer" as (γo [[stid' mtid'] [[s' v'] γs']] reqid) "OfferInv"; rewrite inv_red.
+    iPoseProof ("OfferInv") as "#OfferInv".
+
+    steps_r.
+    iMod ("close" with "[Hs H↦ Hlist ↦offer]") as "_".
+    { rewrite (SLRed_red (f:=syn_stack_inv _ _ _ _ _)). iLeft; iFrame.
+      rewrite /syn_is_offer SLRed_red //.
+      iExists _, _, _; rewrite inv_red //.
+    }
+    sch_yield_ir. steps_r.
+
+    (* Try to take the offer *)
+    iDestruct "OfferInv" as "[OfferInv <-]"; ss. rename γs' into γs.
+    iInv "OfferInv" as "inv" "close"; rewrite SLRed_red.
+    iDestruct "inv" as "[%offerst [↦offerst offer]] /=".
+
+    case_decide; subst.
+    { (* Helping *)
+      iDestruct "offer" as "[offerv offer]".
+      iAssert (emp)%I with "[]" as "E"; first done.
+      iApply (wsim_mem_cas with "↦offerst E");
+        [try prove_inline_cond|try prove_sb_cond|unfold_cris_defs|..]; eauto.
+      iIntros "offer↦ _". iClear "E". case_decide; last done.
+      steps_r. hss_r. steps_r.
+
+      (* Help *)
+      sch_yield_l. force_l true. steps_l.
+      iDestruct "IST" as "[% [% [% [% [[-> ->] [IST [% [% [[-> ->] Help●]]]]]]]]]".
+      iPoseProof (helping_auth_token with "Help● offer") as "%Hreq".
+      iMod (helping_auth_commit with "Help● offer") as "[●offer #◯offer]".
+      iMod ("close" with "[offer↦ ◯offer]") as "_".
+      { iExists 1; iFrame; case_decide; ss. }
+      destruct Hsphelp as [Hfind2 Hfind]; rewrite (Hfind (Helping.help mn) None) //; cycle 1.
+      { rewrite /alist_find eq_rel_dec_correct /=; des_ifs. destruct (dec _ _); ss. }
+      clear Hfind Hfind2.
+      inline_l. steps_l. force_l reqid. steps_l.
+      rewrite /HoareCall_prologue; unseal "Help"; unfold_sp_exact sp SchHdr.yield; ss.
+      force_l (stid, mtid). forces_l. iFrame. iSplit; eauto. steps_l.
+
+      (* Helpee's Atomic Assume *)
+      rewrite /HoareFun_prologue; unseal "Help"; unfold_sp_exact sp SchHdr.yield; ss.
+      steps_l. rename _q1 into stid2, _q2 into mtid2.
+      rewrite /HelpingOn.try_run. steps_l. hss. rewrite Hreq /=.
+      steps_l. rewrite Helping.trans_take. steps_l. clear dependent l. rename _q1 into l'. 
+      steps_l. rewrite Helping.trans_Assume. steps_l.
+      iInv "Hinv" as "StackInv" "Close". rewrite {1}SLRed_red.
+      clear dependent stack_rep offer_rep.
+      iDestruct "StackInv" as "[[%stack_rep [%offer_rep [%l [Hs [H↦ [Hlist Hoffer]]]]]]|[% ●]]";
+        cycle 1.
+      { iExFalso. iCombine "●" "●offer" gives %[WF _]%gmap_view_auth_dfrac_op_valid. ss. }
+      iCombine "Hs ASM'" gives %[->%Excl_included%leibniz_equiv _]%auth_both_valid_discrete.
+      iMod (own_update_2 with "Hs ASM'") as "[Hs Hl]".
+      { eapply auth_update, option_local_update, (exclusive_local_update _ (Excl _)). done. }
+
+      (* Helpee's Atomic Guarantee *)
+      rewrite Helping.trans_Guarantee; force_l; iFrame "Hl". steps_l.
+      rewrite Helping.trans_ret; steps_l.
+
+      (* My Atomic Assume *)
+      iPoseProof (helping_auth_split (1/2) with "●offer") as "[●offer ●reclaim]"; ss.
+      iMod ("Close" with "[●offer]") as "_".
+      { rewrite SLRed_red; iRight; iFrame. }
+      rewrite /HoareFun_epilogue; unseal "Help"; unfold_sp_exact sp SchHdr.yield; ss.
+      forces_l. iDestruct "ASM"  as "[[_ $] _]"; iSplit; eauto. steps_l.
+      rewrite /HoareCall_epilogue; unseal "Help"; unfold_sp_exact sp SchHdr.yield; ss.
+      steps_l. hss.
+      iCombine "Hs ASM'" gives %[->%Excl_included%leibniz_equiv _]%auth_both_valid_discrete. ss.
+      iMod (own_update_2 with "Hs ASM'") as "[Hs Hl]".
+      { eapply auth_update, option_local_update, (exclusive_local_update _ (Excl _)). done. }
+      force_l; iFrame "Hl"; steps_l.
+      iInv "Hinv" as "Hstack" "close".
+      rewrite (SLRed_red (f:=syn_stack_inv _ _ _ _ _)).
+      iDestruct "Hstack" as "[[% [% [% [Hs' _]]]]|[% ●]]".
+      { iExFalso. iCombine "Hs" "Hs'" gives %WF; inv WF. }
+      iPoseProof ("●reclaim" with "●") as "●".
+      iMod ("close" with "[- IST ASM ● offerv]") as "_".
+      { rewrite SLRed_red; iLeft; iFrame. }
+      set (st_src := st_srcL ++ _); set (st_tgt := st_tgtL ++ _).
+      iAssert (IstFull st_src st_tgt)%I with "[● IST]" as "IST".
+      { iExists _, _, _, _; iFrame. iSplit; eauto. }
+      sch_yield_ir. iDestruct "ASM" as "[[_ $] _]".
+      clear st_src st_tgt; iIntros (st_src st_tgt) "IST TID". steps_r.
+
+      iAssert (emp)%I with "[]" as "E"; first done.
+      iApply (wsim_mem_cmp with "E");
+        [try prove_inline_cond|try prove_sb_cond|unfold_cris_defs|..]; eauto.
+      iIntros "_". steps_r. hss_r. steps_r. sch_yield_ir. steps_r. sch_yield_ir. steps_r.
+
+      (* Compare *)
+      iApply (wsim_mem_load with "[offerv]");
+        [try prove_inline_cond|try prove_sb_cond|ss|unfold_cris_defs].
+      iIntros "offerv". steps_r. hss_r. steps_r.
+      sch_yield_ir. steps_r. sch_yield_l. forces_l. iFrame. iSplit; eauto. step. iFrame. done.
+    }
+
+    (* Failed to take the offer - repeat the whole process! *)
+    iApply (wsim_mem_cas _ _ _ _ _ _ _ _ _ _ _ _ _ _ _ _ emp%I with "↦offerst");
+        [try prove_inline_cond|try prove_sb_cond|unfold_cris_defs|..]; eauto.
+    { instantiate (1:=0%Z). destruct (dec _ _); clarify. des_ifs; ss. }
+    iIntros "↦offerst _". steps_r. hss_r. steps_r.
+    iMod ("close" with "[↦offerst offer]") as "_".
+    { iExists _; ss; iFrame. case_decide; clarify. case_decide; eauto. case_decide; clarify. }
+    sch_yield_ir. steps_r.
+
+    iAssert (emp)%I with "[]" as "E"; first done.
+    iApply (wsim_mem_cmp with "E");
+      [try prove_inline_cond|try prove_sb_cond|unfold_cris_defs|..]; eauto.
+    { instantiate (1:=0%Z). destruct (dec _ _); clarify. des_ifs; ss. }
+    iIntros "_". steps_r. hss_r. steps_r. sch_yield_ir. steps_r.
+
+    by_coind CIH. iFrame. done.
+  (*SLOW*)Admitted.
 
   (* Construct ISim.t for summing up each simulation proofs *)
   Lemma sim : ISim.t open StackM StackI init_cond IstFull.
+  Proof.
+    rewrite /StackM /StackI.
+    init_sim.
+    { i; try rewrite /Mod.scopes; s; (hrepeat do 1 unfold_mod); s. apply sub_perm_refl. }
+    { split; first done.
+      iIntros "I"; iExists _, _, [_], [_]; iFrame.
+      admit.
+    }
+    { apply new_stack_simF. }
+    { apply push_simF. }
+    { apply pop_simF. }
   Admitted.
-
-  (* ctxr works as a unit in compositions of module simulations *)
-  (* Lemma ctxr :
-    ctx_refines
-      (StackM.t N ★ MemA.t, emp%I)
-      (StackI.t ★ MemA.t, emp%I).
-  Proof. eapply main_adequacy, sim; eauto. Qed. *)
 End StackIM. End StackIM.
