imp_system/mem/MemA.v
@@ -114,6 +114,20 @@ Section MemRA.
     Persistent (mem_points_to_singleton loc DfracDiscarded v).
   Proof. apply _. Qed.
 
+  Lemma mem_points_to_singleton_agree (loc : mblock * Z) (q1 q2 : dfrac) (v1 v2 : val) :
+    mem_points_to_singleton loc q1 v1 -∗
+    mem_points_to_singleton loc q2 v2 -∗
+    ⌜v1 = v2⌝.
+  Proof.
+    destruct loc.
+    rewrite /mem_points_to_singleton /mem_points_to_singleton_r /=; iIntros "H1 H2".
+    iPoseProof (own_valid_2 with "H1 H2") as "%WF".
+    apply auth_frag_op_valid_1 in WF.
+    rewrite discrete_fun_singleton_op discrete_fun_singleton_valid in WF.
+    rewrite discrete_fun_singleton_op discrete_fun_singleton_valid in WF.
+    rewrite -Some_op Some_valid dfrac_agree_op_valid_L in WF; des; clarify.
+  Qed.
+
   Lemma mem_init_auth_r_valid (csl : string → bool) (genv : GEnv.t) blk ofs v :
     mem_init_val csl genv blk ofs = Some v →
     mem_points_to_singleton_r (blk, ofs) (DfracOwn 1) (Vint v) ≼ mem_init_frag_r csl genv.
